wip

code/experimental/P256/Hacl.Impl.P256.fst
@@ -928,6 +928,7 @@ let uploadOneImpl f =
   upd f (size 2) (u64 0);
   upd f (size 3) (u64 0)
 
+
 let norm p resultPoint tempBuffer = 
   let xf = sub p (size 0) (size 4) in
   let yf = sub p (size 4) (size 4) in 
@@ -940,12 +941,42 @@ let norm p resultPoint tempBuffer =
   let z2f = sub tempBuffer (size 4) (size 4) in 
   let z3f = sub tempBuffer (size 8) (size 4) in
   let tempBuffer20 = sub tempBuffer (size 12) (size 20) in 
-  
-  Hacl.Spec.P256.MontgomeryMultiplication.montgomery_multiplication_buffer zf zf z2f;
-  Hacl.Spec.P256.MontgomeryMultiplication.montgomery_multiplication_buffer z2f zf z3f;
 
+    let h0 = ST.get() in 
+  Hacl.Spec.P256.MontgomeryMultiplication.montgomery_multiplication_buffer zf zf z2f;
+    let h1 = ST.get() in 
+    assert(as_seq h1 z2f == montgomery_multiplication_seq (as_seq h0 zf) (as_seq h0 zf));
+    
+    assert(felem_seq_as_nat (montgomery_multiplication_seq (as_seq h0 zf) (as_seq h0 zf)) = toDomain_ (fromDomain_ (
+    felem_seq_as_nat (as_seq h0 zf)) * fromDomain_ (felem_seq_as_nat (as_seq h0 zf)) % prime));
+    
+    assert(felem_seq_as_nat (as_seq h1 z2f) = toDomain_ (fromDomain_ (
+    felem_seq_as_nat (as_seq h0 zf)) * fromDomain_ (felem_seq_as_nat (as_seq h0 zf)) % prime));
+
+    assert(as_nat h1 z2f = toDomain_ (fromDomain_ (as_nat h0 zf) * fromDomain_ (as_nat h0 zf) % prime));
+
+  Hacl.Spec.P256.MontgomeryMultiplication.montgomery_multiplication_buffer z2f zf z3f;
+    let h2 = ST.get() in  
+    assert(as_seq h2 z3f == montgomery_multiplication_seq (as_seq h1 z2f) (as_seq h0 zf));
+    assert(as_nat h2 z3f == toDomain_ (fromDomain_ (as_nat h1 z2f) * fromDomain_ (as_nat h0 zf) % prime));
+    assert(as_nat h2 z3f == toDomain_ (fromDomain_ (toDomain_ (fromDomain_ (as_nat h0 zf) * fromDomain_ (as_nat h0 zf) % prime)) * fromDomain_ (as_nat h0 zf) % prime));
+    let open Hacl.Spec.P256.Normalisation in 
+      lemma_1 (fromDomain_ (as_nat h0 zf));
+      assert(let z = fromDomain_ (as_nat h0 zf) in as_nat h2 z3f == toDomain_ (z * z * z % prime));
+      assert(let z = fromDomain_ (as_nat h0 zf) in as_nat h2 z2f == toDomain_ (z * z % prime));
   Hacl.Spec.P256.MontgomeryMultiplication.exponent z2f z2f tempBuffer20;
+    let h3 = ST.get() in 
+    assert(let k = fromDomain_ (as_nat h2 z2f) in as_nat h3 z2f = toDomain_ ((pow k (prime - 2)) % prime));
+    assert(let k = fromDomain_ (as_nat h0 zf) * fromDomain_ (as_nat h0 zf) % prime in as_nat h3 z2f = toDomain_ ((pow k (prime - 2)) % prime));
+    (* power distributivity *)
+    assume(let k = fromDomain_ (as_nat h0 zf) * fromDomain_ (as_nat h0 zf) in as_nat h3 z2f = toDomain_ ((pow k (prime - 2)) % prime));
   Hacl.Spec.P256.MontgomeryMultiplication.exponent z3f z3f tempBuffer20;
+    let h4 = ST.get() in 
+    assert(let k = fromDomain_ (as_nat h3 z3f) in as_nat h4 z3f = toDomain_ ((pow k (prime - 2)) % prime));
+    admit();
+    let h4 = ST.get() in 
+    assert(let k = fromDomain_ (as_nat h3 z3f) in as_nat h4 z3f = toDomain_ ((pow k (prime - 2)) % prime));
+    admit();
 
   Hacl.Spec.P256.MontgomeryMultiplication.montgomery_multiplication_buffer xf z2f z2f;
   Hacl.Spec.P256.MontgomeryMultiplication.montgomery_multiplication_buffer yf z3f z3f;
