code/experimental/P256/Hacl.Spec.P256.Chain.fst
@@ -1,0 +1,64 @@
+module Hacl.Spec.P256.Chain
+
+open FStar.HyperStack.All
+open FStar.HyperStack
+open FStar.HyperStack.ST
+
+module ST = FStar.HyperStack.ST
+module HS = FStar.HyperStack
+
+open Lib.IntTypes
+open Lib.Buffer
+
+open Hacl.Impl.Curve25519.Field64.Core
+module C =  Hacl.Spec.Curve25519.Field64.Core
+module D = Hacl.Spec.Curve25519.Field64.Definition
+open  Hacl.Spec.P256.Core
+open Hacl.Spec.P256.Lemmas
+open Hacl.Spec.P256.Definitions
+open Hacl.Spec.P256.SolinasReduction
+open Hacl.Spec.P256.MontgomeryMultiplication
+open Hacl.Spec.P256.MontgomeryMultiplication.PointDouble
+open Hacl.Spec.P256.MontgomeryMultiplication.PointAdd
+
+
+open Lib.Loops
+open FStar.Math.Lemmas
+
+module B = LowStar.Buffer
+open FStar.Mul
+
+
+open Hacl.Impl.P256
+
+val chain: p: point_prime -> tempBuffer: lbuffer uint64 (size 100) ->  Stack unit
+  (requires fun h -> True)
+  (ensures fun h0 _ h1 -> True)
+
+let chain p tempBuffer = 
+  let tempBuffer32 = sub tempBuffer (size 0) (size 32) in 
+  let tempBuffer88 = sub tempBuffer (size 0) (size 88) in 
+
+  let tempBufferPoint = sub tempBuffer (size 88) (size 12) in 
+
+    let h0 = ST.get() in 
+  pointToDomain p p;
+    let h1 = ST.get() in
+    assert(point_x_as_nat h1 p == toDomain_ (point_x_as_nat h0 p) /\ point_y_as_nat h1 p == toDomain_ (point_x_as_nat h0 p) /\ point_z_as_nat h1 p == toDomain_ (point_z_as_nat h0 p) );
+  point_double p p tempBuffer88;
+    let h2 = ST.get() in 
+    assert(as_seq #MUT #uint64 #12 h2 p == point_double_seq (as_seq #MUT #uint64 #12 h1 p));
+    assert(
+      let x = toDomain_ (point_x_as_nat h0 p) in 
+      let y = toDomain_ (point_y_as_nat h0 p) in 
+      let z = toDomain_ (point_z_as_nat h0 p) in 
+      let xD = fromDomain_ x in let yD = fromDomain_ y in let zD = fromDomain_ z  in 
+      let (xN, yN, zN) = _point_double (point_x_as_nat h0 p, point_y_as_nat h0 p, point_z_as_nat h0 p) in 
+      point_x_as_nat h2 p == toDomain_ (xN) (*/\ point_y_as_nat h2 p == toDomain_ (yN) /\ point_z_as_nat h2 p == toDomain_ (zN)*));
+
+   assert(let x = point_x_as_nat h1 p in let y = point_y_as_nat h1 p in let z = point_z_as_nat h1 p in let xD = fromDomain_ x in let yD = fromDomain_ y in let zD = fromDomain_ z  in 
+  let (xN, yN, zN) = _point_double (xD, yD, zD) in 
+  point_x_as_nat h2 p == toDomain_ (xN) (*/\ point_y_as_nat h2 p == toDomain_ (yN) /\ point_z_as_nat h2 p == toDomain_ (zN)*));
+    
+()    
+  
