code/experimental/P256/Hacl.Spec.P256.Normalisation.fst
@@ -1,0 +1,44 @@
+module Hacl.Spec.P256.Normalisation
+
+
+open FStar.HyperStack.All
+open FStar.HyperStack
+open FStar.HyperStack.ST
+
+module ST = FStar.HyperStack.ST
+module HS = FStar.HyperStack
+
+open Lib.IntTypes
+open Lib.Buffer
+
+open Hacl.Impl.Curve25519.Field64.Core
+module C =  Hacl.Spec.Curve25519.Field64.Core
+module D = Hacl.Spec.Curve25519.Field64.Definition
+open  Hacl.Spec.P256.Core
+open Hacl.Spec.P256.Lemmas
+open Hacl.Spec.P256.Definitions
+open Hacl.Spec.P256.MontgomeryMultiplication
+
+
+open Lib.Loops
+open FStar.Math.Lemmas
+
+module B = LowStar.Buffer
+
+
+let _norm p =
+  let open FStar.Mul in 
+  let (x, y, z) = p in
+  let z2 = z * z % prime in 
+  let z2i = modp_inv2 z in 
+  let z3 = z * z *  z % prime in 
+  let z3i = modp_inv2 z3 in 
+  let x3 = (x * z2i) % prime in 
+  let y3 = (y * z3i) % prime in 
+  let z3 = 1 in 
+  (x3, y3, z3)
+
+open FStar.Mul
+
+(* z * z * pow2 256 * z % prime *)
+val lemma_1: z: nat-> Lemma (toDomain_ (fromDomain_ ((z * z % prime) * pow2 256 % prime) * z % prime) == toDomain_ (z * z * z % prime)) 
